internal/Notations.v
@@ -3,5 +3,6 @@ Reserved Notation "x ‘‘→’’ y" (at level 99, right associativity, y at 
 Reserved Notation "x ‘→’ y" (at level 99, right associativity, y at level 200).
 Reserved Notation "x ‘’ y" (at level 15, left associativity).
 Reserved Notation "Γ ▻ x" (at level 55, right associativity).
+Reserved Notation "Γ ▻▻ Γ'" (at level 60, right associativity).
 Reserved Notation "□ T" (at level 0).
 Reserved Notation "x [ 0 ↦ y ]" (at level 0, no associativity).
